Examples/EBLin.v
@@ -1,0 +1,56 @@
+From LHL.Core Require Import
+  Linearizability
+  LogicFacts
+  Traces
+  Specs
+  Program
+  Tensor
+  LinFacts.
+
+From LHL.Examples Require Import
+  CASSpec
+  ExchangerSpec
+  Exchanger
+  ElimArray
+  EBStack
+  NameSpec
+  RandomSpec
+  WaitFreeStackSpec
+  AtomicStackSpec
+  ArraySpec
+  Array.
+
+Infix "⊗" := tensorSpec (at level 40).
+
+Theorem ExchLin {T A} :
+  Lin (T:=T)
+    (overObj ((nameSpec ⊗ casSpec) :> exchImpl (A:=A)))
+    exchSpec.
+eapply soundness.
+apply oneCellExchCorrect.
+Qed.
+
+Theorem ElimArrLin {T A} :
+  Lin (T:=T)
+    (overObj ((randSpec ⊗ arraySpec T exchSpec) :> elimArray T A)) exchSpec.
+eapply soundness.
+apply elimArrayCorrect.
+Qed.
+
+Definition arrEBImpl T A :
+  Impl
+    ((RandSig |+| ArraySig (CASSig (option A)) T) |+| WaitFreeStackSig A)
+    (AtomicStackSig A)
+:=
+  tensorImpl
+    (arrayImpl
+    |> elimArray T (option A))
+    idImpl 
+  |> EBStack A.
+
+Theorem EBLin {T A} :
+  Lin (T:=T)
+    (overObj
+      (((ntensor (nameSpec ⊗ casSpec) T) ⊗ wfStackSpec) :>
+      (tensorImpl (elimArray T A) idImpl |> EBStack A)))
+    atomicStackSpec.
