README.md
@@ -1,27 +1,25 @@
 # LHL
- 
- Steps I took to setup:
 
- ```
- opam init
- eval $(opam env)
- opam update
- opam switch create LHL 4.13.1
- opam pin add coq 8.18.0
-```
+Linearizability Hoare Logic -- a sound and complete program logic for compositional linearizability.
 
-For VsCoq:
-```
-opam install vscoq-language-server
-```
+## Setup Steps
 
-Generating Coq Makefile:
+Compiled with Coq version 8.18.0, OCaml version 5.2.0.
+
+We are using make. To build the project:
 ```
 coq_makefile -f _CoqProject -o Makefile
+make
 ```
 
-To Install Paco
+You will also need to install Paco to compile this project. Install like so:
 ```
 opam repo add coq-released https://coq.inria.fr/opam/released
 opam install coq-paco
 ```
+
+## Usage
+
+The program logic is defined in `Logic.v`. Import this along with `Program` and `ProgramRules.v` to get the typical control flow constructs along with their derived rules. Modules are of type `Impl` -- once you define a module, you may verify it with he toplevel program logic judgement `VerifyImpl`. After this, you may import `LogicFacts.v` and use `soundness` to derive a linearizability proof.
+
+From here, you may verify modules and compose them together using the theorems in `LinFacts.v`. `obs_ref` gives you vertical composition, and `locality` gives you horizontal composition.
